lectures/Lowstar/code/RevString.fst
@@ -1,0 +1,26 @@
+module RevString
+
+open FStar.List.Tot
+open FStar.Seq
+
+let rec rev_list l =
+  match l with
+  | [] -> []
+  | h::t -> rev_list t @ [h]
+
+val swap : #a:eqtype -> s:seq a -> i:nat{i < Seq.length s} -> j:nat{j < Seq.length s} -> seq a
+let swap s i j =
+  let ei = Seq.index s i in
+  let ej = Seq.index s j in
+  let s' = Seq.upd s i ej in
+  Seq.upd s' j ei
+
+val rev_seq' : #a:eqtype -> s:seq a -> i:nat{i <= Seq.length s} -> Tot (seq a) (decreases (Seq.length s - i))
+let rec rev_seq' s i =
+  if i < Seq.length s / 2 then
+    let s' = swap s i (Seq.length s - i - 1) in
+    rev_seq' s' (i + 1)
+  else
+    s
+
+let rev_seq s = rev_seq' s 0
